Using the new-style simulations
git-svn-id: https://yquem.inria.fr/compcert/svn/compcert/branches/new-simulations@1666 fca1b0fc-160b-0410-b1d3-a4f43f01ea2e

cfrontend/Csem.v
@@ -1185,5 +1185,5 @@ Inductive final_state: state -> int -> Prop :=
 (** Wrapping up these definitions in a small-step semantics. *)
 
 Definition semantics (p: program) :=
-  mk_semantics step (initial_state p) final_state (Genv.globalenv p).
+  Semantics step (initial_state p) final_state (Genv.globalenv p).
 
